More parametricity exercises

theories/parametricity.v
@@ -3,29 +3,29 @@ From tutorial_popl20 Require Export safety.
 Section parametricity.
   Context `{heapG Σ}.
 
-  (* REMOVE *) Definition exercise5_sem_ty Σ (v : val) : sem_ty Σ :=
+  (* REMOVE *) Definition identity_param_sem_ty Σ (v : val) : sem_ty Σ :=
     SemTy (λ w, ⌜w = v⌝)%I.
 
-  Lemma exercise5 `{!heapPreG Σ} e (v : val) σ w es σ' :
+  Lemma identity_param `{!heapPreG Σ} e (v : val) σ w es σ' :
     (∀ `{heapG Σ}, ∅ ⊨ e : ∀ A, A → A) →
     rtc erased_step ([e <_> v]%E, σ) (of_val w :: es, σ') → w = v.
   (* REMOVE *) Proof.
     intros He.
     apply sem_gen_type_safety with (φ := λ u, u = v)=> ?.
-    exists (exercise5_sem_ty Σ v). split.
+    exists (identity_param_sem_ty Σ v). split.
     { by iIntros (?) "?". }
     iIntros (vs) "!# #Hvs".
     iPoseProof (He with "Hvs") as "He /=".
     wp_apply (wp_wand with "He").
     iIntros (u) "#Hu".
-    iSpecialize ("Hu" $! (exercise5_sem_ty Σ v)).
+    iSpecialize ("Hu" $! (identity_param_sem_ty Σ v)).
     wp_apply (wp_wand with "Hu"). iIntros (w') "Hw'". by iApply "Hw'".
   Qed.
 
-  (* REMOVE *) Definition exercise6_sem_ty Σ : sem_ty Σ :=
+  (* REMOVE *) Definition empty_type_param_sem_ty Σ : sem_ty Σ :=
     SemTy (λ w, False)%I.
 
-  Lemma exercise6 `{!heapPreG Σ} e (v : val) σ w es σ' :
+  Lemma empty_type_param `{!heapPreG Σ} e (v : val) σ w es σ' :
     (∀ `{heapG Σ}, ∅ ⊨ e : ∀ A, A) →
     rtc erased_step ([e <_>]%E, σ) (of_val w :: es, σ') →
     False.
@@ -33,12 +33,112 @@ Section parametricity.
     intros He.
     change False with ((λ _, False) w).
     apply sem_gen_type_safety with (φ := λ _, False)=> ?.
-    exists (exercise6_sem_ty Σ). split.
+    exists (empty_type_param_sem_ty Σ). split.
     { by iIntros (?) "?". }
     iIntros (vs) "!# #Hvs".
     iPoseProof (He with "Hvs") as "He /=".
     wp_apply (wp_wand with "He").
     iIntros (u) "#Hu".
-    iApply ("Hu" $! (exercise6_sem_ty Σ)).
+    iApply ("Hu" $! (empty_type_param_sem_ty Σ)).
   Qed.
+
+  (* REMOVE *) Definition boolean_param_sem_ty Σ (v1 v2 : val) : sem_ty Σ :=
+    SemTy (λ w, ⌜w = v1 ∨ w = v2⌝)%I.
+
+  Lemma boolean_param `{!heapPreG Σ} e (v1 v2 : val) σ w es σ' :
+    (∀ `{heapG Σ}, ∅ ⊨ e : ∀ A, A → A → A) →
+    rtc erased_step ([e <_> v1 v2]%E, σ) (of_val w :: es, σ') → w = v1 ∨ w = v2.
+  (* REMOVE *) Proof.
+    intros He.
+    apply sem_gen_type_safety with (φ := λ w, w = v1 ∨ w = v2)=> ?.
+    exists (boolean_param_sem_ty Σ v1 v2). split.
+    { by iIntros (?) "?". }
+    iIntros (vs) "!# #Hvs".
+    iPoseProof (He with "Hvs") as "He /=".
+    wp_apply (wp_wand with "He").
+    iIntros (u) "#Hu".
+    iSpecialize ("Hu" $! (boolean_param_sem_ty Σ v1 v2)).
+    wp_apply (wp_wand with "Hu"). iIntros (w') "#Hw'".
+    iSpecialize ("Hw'" $! v1 with "[]"); first by eauto.
+    wp_apply (wp_wand with "Hw'").
+    iIntros (w'') "#Hw''".
+    by iApply ("Hw''" $! v2 with "[]"); eauto.
+  Qed.
+
+  (* REMOVE *) Definition nat_param_sem_ty Σ : sem_ty Σ :=
+    SemTy (λ w, ∃ n : nat, ⌜w = #n⌝)%I.
+
+  Lemma nat_param `{!heapPreG Σ} e σ w es σ' :
+    (∀ `{heapG Σ}, ∅ ⊨ e : ∀ A, (A → A) → A → A) →
+    rtc erased_step ([e <_> (λ: "n", "n" + #1)%V #0]%E, σ)
+        (of_val w :: es, σ') → ∃ n : nat, w = #n.
+  (* REMOVE *) Proof.
+    intros He.
+    apply sem_gen_type_safety with (φ := λ w, ∃ n : nat, w = #n)=> ?.
+    exists (nat_param_sem_ty Σ). split.
+    { iIntros (?). iDestruct 1 as (?) "%". eauto. }
+    iIntros (vs) "!# #Hvs".
+    iPoseProof (He with "Hvs") as "He /=".
+    wp_apply (wp_wand with "He").
+    iIntros (u) "#Hu".
+    iSpecialize ("Hu" $! (nat_param_sem_ty Σ)).
+    wp_apply (wp_wand with "Hu"). iIntros (w') "#Hw'".
+    iSpecialize ("Hw'" $! (λ: "n", "n" + #1)%V with "[]").
+    { iIntros "!#" (? [n ->]).
+      wp_lam.
+      wp_op.
+      iExists (n + 1)%nat.
+      by rewrite Nat2Z.inj_add. }
+    wp_apply (wp_wand with "Hw'").
+    iIntros (w'') "#Hw''".
+    iApply ("Hw''" $! #0 with "[]"); eauto.
+    by iExists 0%nat.
+  Qed.
+
+  (* REMOVE *) Definition strong_nat_param_sem_ty Σ (ψ : nat → val → Prop) : sem_ty Σ :=
+    SemTy (λ w, ∃ n : nat, ⌜ψ n w⌝)%I.
+
+  Definition strong_nat_param_semtyp_family
+             {A Σ} (Ψ : A → sem_ty Σ) : sem_ty Σ :=
+    SemTy (λ w, ∃ n, Ψ n w)%I.
+
+  Lemma strong_nat_param `{!heapPreG Σ} e σ w es σ' (f z : val) ψ:
+    (∀ `{heapG Σ}, ∅ ⊨ e : ∀ A, (A → A) → A → A) →
+    (∀ `{heapG Σ},
+        ∃ (Ψ : nat → sem_ty Σ),
+          (∀ n w, Ψ n w -∗ ⌜ψ n w⌝) ∧
+          (∀ n w, {{{Ψ n w}}} f w {{{w', RET w'; Ψ (S n) w'}}}) ∧
+          (Ψ 0%nat z)%I) →
+    rtc erased_step ([e <_> f z]%E, σ) (of_val w :: es, σ') → ∃ n : nat, ψ n w.
+  (* REMOVE *) Proof.
+    intros He Hfz.
+    apply sem_gen_type_safety with (φ := λ w, ∃ n, ψ n w)=> ?.
+    exists (strong_nat_param_sem_ty Σ ψ). split.
+    { iIntros (?). iDestruct 1 as (?) "%". eauto. }
+    specialize (Hfz _) as (Ψ & HΨ & Hf & Hz).
+    iIntros (vs) "!# #Hvs".
+    iPoseProof (He with "Hvs") as "He /=".
+    wp_apply (wp_wand with "He").
+    iIntros (u) "#Hu".
+    iSpecialize ("Hu" $! (strong_nat_param_semtyp_family Ψ)).
+    wp_apply (wp_wand with "Hu"). iIntros (w') "#Hw'".
+    iSpecialize ("Hw'" $! f with "[]").
+    { iIntros "!#" (u') "Hu'".
+      iDestruct "Hu'"as (k) "Hu'".
+      iApply (Hf with "Hu'").
+      iNext.
+      iIntros (u'') "Hu''".
+      by iExists _. }
+    wp_apply (wp_wand with "Hw'").
+    iIntros (w'') "#Hw''".
+    iApply wp_wand.
+    { iApply ("Hw''" $! z with "[]"); eauto.
+      iExists 0%nat.
+      iApply Hz. }
+    iIntros (v).
+    iDestruct 1 as (k) "Hv".
+    iExists k.
+    by iApply HΨ.
+  Qed.
+
 End parametricity.
